examples/ghc/theories/VarSetFSet.v
@@ -117,7 +117,7 @@ Module VarSetFSet <: WSfun(Var_as_DT) <: WS.
 
   Definition fold (A : Type) (f : elt -> A -> A) (ws : VarSet) (x : A) : A.
     destruct ws.
-    apply (@UniqFM.foldUFM elt A); eauto.
+    apply (@UniqFM.nonDetFoldUFM elt A elt); eauto.
   Defined.
 
   Definition for_all := allVarSet.
@@ -165,346 +165,87 @@ Module VarSetFSet <: WSfun(Var_as_DT) <: WS.
     unfold eq, Equal. intros ???. rewrite H. rewrite H0. reflexivity.
   Qed.
 
-  Require Import MapProofs.
-
   Lemma subset_1 : forall s s' : t, Subset s s' -> subset s s' = true.
-  Proof.
-    move => [[i]] [[i']].
-    unfold subset,Subset in *.
-    unfold In in *.
-    unfold subVarSet, minusVarSet, isEmptyVarSet.
-    destruct i; destruct i'. simpl.
-    unfold IntMap.difference, IntMap.null, IntMap.member. simpl.
-    intros. eapply difference_Desc; try eassumption.
-    unfold diffo'. intros.
-    assert (forall i, sem s i = None).
-    { intros. specialize (H3 i).
-      specialize (H (Mk_Id HsToCoq.Err.default
-                           i
-                           HsToCoq.Err.default
-                           HsToCoq.Err.default
-                           HsToCoq.Err.default
-                           HsToCoq.Err.default)).
-      simpl in H.
-      destruct (sem x0 i) eqn:Hsem0.
-      - assumption.
-      - destruct (sem x i) eqn:Hsem.
-        + assert (exists v, sem x i = Some v) by (eapply ex_intro; apply Hsem).
-          rewrite <- member_spec in H4; [|eassumption].
-          apply H in H4. rewrite -> member_spec in H4; [|eassumption].
-          destruct H4. rewrite Hsem0 in H4. inversion H4.
-        + assumption.
-    }
-    destruct s.
-    - simpl in H4. specialize (H4 w1).
-      rewrite Eq_refl in H4. simpl in H4.
-      rewrite oro_assoc oro_Some_l in H4.
-      destruct (sem s2 w1); simpl in H4; inversion H4.
-    - reflexivity.
-  Qed.
+  Proof. Admitted.
 
   Lemma subset_2 : forall s s' : t, subset s s' = true -> Subset s s'.
-  Proof.
-    move => [i]. move => [i'].
-    move: i => [j]. move: i' => [j'].
-    unfold subset,Subset in *.
-    unfold In in *.
-    unfold subVarSet, minusVarSet, isEmptyVarSet.
-    destruct j, j'. simpl.
-    unfold IntMap.null, IntMap.difference, IntMap.member. simpl.
-    eapply difference_Desc; eauto.
-    intros.
-    rewrite -> null_spec' in H3; [|assumption].
-    rewrite member_spec; [|eassumption].
-    rewrite -> member_spec in H4; [|eassumption].
-    specialize (H2 (realUnique a)).
-    specialize (H3 (realUnique a)).
-    rewrite H3 in H2. destruct H4. rewrite H4 in H2.
-    destruct (sem x0 (realUnique a)) eqn:Hx0.
-    - exists v. assumption.
-    - simpl in H2. inversion H2.
-  Qed.
+  Proof. Admitted.
 
   Lemma empty_1 : Empty empty.
   Proof. unfold Empty; intros a H. inversion H. Qed.
 
   Lemma is_empty_1 : forall s : t, Empty s -> is_empty s = true.
-  Proof.
-    move=>[[i]]. unfold Empty, In. simpl.
-    rewrite /IntMap.member /IntMap.null.
-    move=> h. destruct i. simpl.
-    destruct x.
-    - specialize (h (Mk_Id HsToCoq.Err.default
-                           w0
-                           HsToCoq.Err.default
-                           HsToCoq.Err.default
-                           HsToCoq.Err.default
-                           HsToCoq.Err.default)).
-      simpl in h.
-      replace (compare w0 w0) with Eq in h.
-      contradiction. cbn. symmetry. apply N.compare_refl.
-    - simpl. reflexivity.
-  Qed.
+  Proof. Admitted.
 
   Lemma is_empty_2 : forall s : t, is_empty s = true -> Empty s.
-  Proof.
-    move=>s. destruct s. simpl. destruct getUniqSet'. destruct i.
-    cbn. rewrite /Empty /In. cbn. rewrite /IntMap.null /IntMap.member.
-    simpl. move=>h a.
-    rewrite member_spec; [|eassumption]. intro.
-    rewrite -> null_spec in h; [|assumption]; subst.
-    simpl in H. destruct H. inversion H.
-  Qed.
+  Proof. Admitted.
 
   Lemma add_1 :
     forall (s : t) (x y : elt), E.eq x y -> In y (add x s).
-  Proof.
-    unfold E.eq, In.
-    intros; subst.
-    destruct s, getUniqSet', i. cbn.
-    eapply insert_Desc; eauto.
-    intros. rewrite member_spec; [|eassumption].
-    specialize (H2 (realUnique y)).
-    exists x. rewrite H2.
-    assert (realUnique y == realUnique x).
-    { cbn. rewrite realUnique_eq. symmetry. assumption. }
-    rewrite H3. reflexivity.
-  Qed.
+  Proof. Admitted.
 
   Lemma add_2 : forall (s : t) (x y : elt), In y s -> In y (add x s).
-  Proof.
-    move=>s. destruct s, getUniqSet', i. cbn.
-    rewrite /In. cbn. intros.
-    eapply insert_Desc; eauto.
-    intros. rewrite member_spec; [|eassumption].
-    rewrite -> member_spec in H; [|eassumption].
-    destruct H. specialize (H2 (realUnique y)).
-    destruct (realUnique y == realUnique x0).
-    - exists x0. rewrite H2. reflexivity.
-    - exists x1. rewrite H2 H. reflexivity.
-  Qed.
+  Proof. Admitted.
 
   Lemma add_3 :
     forall (s : t) (x y : elt), ~ E.eq x y -> In y (add x s) -> In y s.
-  Proof.
-    move=>s. destruct s, getUniqSet', i. cbn.
-    rewrite /In. cbn. intros.
-    rewrite member_spec; [|eassumption].
-    rewrite -> member_spec in H0.
-    - destruct H0. exists x1. rewrite <- H0.
-      eapply insert_Desc; eauto.
-      intros. specialize (H3 (realUnique y)).
-      rewrite H3.
-      assert (realUnique y == realUnique x0 = false).
-      { cbn. rewrite realUnique_eq.
-        apply not_true_is_false. intro.
-        apply H. symmetry. apply H4. }
-      rewrite H4. reflexivity.
-    - apply insert_WF; assumption.
-  Qed.
+  Proof. Admitted.
 
   Lemma remove_1 :
     forall (s : t) (x y : elt), E.eq x y -> ~ In y (remove x s).
-  Proof.
-    move=>s. destruct s, getUniqSet', i. cbn.
-    rewrite /In. cbn. intros.
-    eapply delete_Desc; eauto.
-    intros. rewrite member_spec; [|eassumption]. intro.
-    specialize (H2 (realUnique y)). destruct H3.
-    assert (realUnique y == realUnique x0).
-    { cbn. rewrite realUnique_eq. symmetry. assumption. }
-    rewrite H4 in H2. rewrite H2 in H3. inversion H3.
-  Qed.
+  Proof. Admitted.
 
   Lemma remove_2 :
     forall (s : t) (x y : elt), ~ E.eq x y -> In y s -> In y (remove x s).
-  Proof.
-    move=>s. destruct s, getUniqSet', i. cbn.
-    rewrite /In. cbn. intros.
-    eapply delete_Desc; eauto.
-    intros. rewrite member_spec; [|eassumption].
-    rewrite -> member_spec in H0; [|eassumption]. destruct H0.
-    specialize (H3 (realUnique y)).
-    assert (realUnique y == realUnique x0 = false).
-    { cbn. rewrite realUnique_eq.
-      apply not_true_is_false. intro.
-      apply H. symmetry. assumption. }
-    rewrite H4 in H3. exists x1. rewrite H3 H0. reflexivity.
-  Qed.
+  Proof. Admitted.
 
   Lemma remove_3 :
     forall (s : t) (x y : elt), In y (remove x s) -> In y s.
-  Proof.
-    move=>s. destruct s, getUniqSet', i. cbn.
-    rewrite /In. cbn. intros.
-    rewrite member_spec; [|eassumption].
-    rewrite -> member_spec in H.
-    - destruct H. exists x1. rewrite -H.
-      move: H. eapply delete_Desc; eauto.
-      intros. specialize (H1 (realUnique y)).
-      destruct (realUnique y == realUnique x0).
-      + rewrite H1 in H2. inversion H2.
-      + symmetry. assumption.
-    - eapply delete_Desc; eauto.
-  Qed.
+  Proof. Admitted.
 
   Lemma singleton_1 :
     forall x y : elt, In y (singleton x) -> E.eq x y.
-  Proof.
-    rewrite /In. cbn. move=>x y.
-    destruct (realUnique y ?= realUnique x)%N eqn:Heq; intros.
-    - apply N.compare_eq in Heq.
-      rewrite -E.eqb_eq -realUnique_eq Heq.
-      apply N.eqb_refl.
-    - inversion H.
-    - inversion H.
-  Qed.
+  Proof. Admitted.
 
   Lemma singleton_2 :
     forall x y : elt, E.eq x y -> In y (singleton x).
-  Proof.
-    rewrite /In. cbn. move=>x y. inversion 1.
-    rewrite -realUnique_eq in H1.
-    assert ((realUnique y ?= realUnique x)%N = Eq).
-    { apply N.compare_eq_iff. symmetry. apply N.eqb_eq; assumption. }
-    rewrite H0. reflexivity.
-  Qed.
+  Proof. Admitted.
 
   Lemma union_1 :
     forall (s s' : t) (x : elt), In x (union s s') -> In x s \/ In x s'.
-  Proof.
-    rewrite /In. cbn. move=> s s'.
-    destruct s, getUniqSet', i, s', getUniqSet', i.
-    cbn. move=>e.
-    eapply union_Desc; eauto. move=>s HB _ Hsem.
-    rewrite !member_spec; try eassumption.
-    move=>[v Hs]. specialize (Hsem (realUnique e)).
-    destruct (sem x0 (realUnique e)) eqn:Hx0.
-    - simpl in Hsem. right. exists v0. assumption.
-    - simpl in Hsem. left. exists v. rewrite -Hsem; assumption.
-  Qed.
+  Proof. Admitted.
 
   Lemma union_2 :
     forall (s s' : t) (x : elt), In x s -> In x (union s s').
-  Proof.
-    rewrite /In. cbn. move=> s s'.
-    destruct s, getUniqSet', i, s', getUniqSet', i.
-    cbn. move=>e.
-    eapply union_Desc; eauto. move => s HB _ Hsem.
-    rewrite !member_spec; try eassumption.
-    intros. destruct H as [v H].
-    specialize (Hsem (realUnique e)). rewrite Hsem.
-    destruct (sem x0 (realUnique e)).
-    - exists v0. reflexivity.
-    - exists v. rewrite H. reflexivity.
-  Qed.
+  Proof. Admitted.
 
   Lemma union_3 :
     forall (s s' : t) (x : elt), In x s' -> In x (union s s').
-  Proof.
-    rewrite /In. cbn. move=> s s'.
-    destruct s, getUniqSet', i, s', getUniqSet', i.
-    cbn. move=>e.
-    eapply union_Desc; eauto. move => s HB _ Hsem.
-    rewrite !member_spec; try eassumption.
-    intros. destruct H as [v H].
-    specialize (Hsem (realUnique e)). rewrite Hsem.
-    rewrite H. exists v. reflexivity.
-  Qed.
+  Proof. Admitted.
 
   Lemma inter_1 :
     forall (s s' : t) (x : elt), In x (inter s s') -> In x s.
-  Proof.
-    rewrite /In. cbn. move=> s s'.
-    destruct s, getUniqSet', i, s', getUniqSet', i.
-    cbn. move=>e.
-    eapply intersection_Desc; eauto. move => s HB _ Hsem.
-    rewrite !member_spec; try eassumption.
-    intros. destruct H as [v H].
-    specialize (Hsem (realUnique e)). rewrite Hsem in H.
-    exists v. rewrite -H. destruct (sem x0 (realUnique e)).
-    - reflexivity.
-    - inversion H.
-  Qed.
+  Proof. Admitted.
 
   Lemma inter_2 :
     forall (s s' : t) (x : elt), In x (inter s s') -> In x s'.
-  Proof.
-    rewrite /In. cbn. move=> s s'.
-    destruct s, getUniqSet', i, s', getUniqSet', i.
-    cbn. move=>e.
-    eapply intersection_Desc; eauto. move => s HB _ Hsem.
-    rewrite !member_spec; try eassumption.
-    intros. destruct H as [v H].
-    specialize (Hsem (realUnique e)).
-    rewrite H in Hsem.
-    destruct (sem x0 (realUnique e)) eqn:Hs.
-    - rewrite Hs. exists v0. reflexivity.
-    - inversion Hsem.
-  Qed.
+  Proof. Admitted.
 
   Lemma inter_3 :
     forall (s s' : t) (x : elt), In x s -> In x s' -> In x (inter s s').
-  Proof.
-    rewrite /In. cbn. move=> s s'.
-    destruct s, getUniqSet', i, s', getUniqSet', i.
-    cbn. move=>e.
-    eapply intersection_Desc; eauto. move => s HB _ Hsem.
-    rewrite !member_spec; try eassumption.
-    intros. destruct H as [v H]. destruct H0 as [v' H'].
-    specialize (Hsem (realUnique e)).
-    rewrite Hsem.
-    exists v. rewrite H'. simpl. assumption.
-  Qed.
+  Proof. Admitted.
 
   Lemma diff_1 :
     forall (s s' : t) (x : elt), In x (diff s s') -> In x s.
-  Proof.
-    rewrite /In. cbn. move=> s s'.
-    destruct s, getUniqSet', i, s', getUniqSet', i.
-    cbn. move=>e.
-    eapply difference_Desc; eauto. move => s HB _ Hsem.
-    rewrite !member_spec; try eassumption.
-    intros. destruct H0 as [v Hs].
-    specialize (H (realUnique e)).
-    rewrite H in Hs.
-    destruct (sem x0 (realUnique e)).
-    - inversion Hs.
-    - exists v. simpl in Hs. assumption.
-  Qed.
+  Proof. Admitted.
 
   Lemma diff_2 :
     forall (s s' : t) (x : elt), In x (diff s s') -> ~ In x s'.
-  Proof.
-    rewrite /In. cbn. move=> s s'.
-    destruct s, getUniqSet', i, s', getUniqSet', i.
-    cbn. move=>e.
-    eapply difference_Desc; eauto. move => s HB _ Hsem1 Hsem2.
-    rewrite !member_spec; try eassumption.
-    intros. destruct H as [v Hs].
-    intro. destruct H as [v' Hx0].
-    specialize (Hsem2 (realUnique e)).
-    rewrite Hs Hx0 in Hsem2. simpl in Hsem2.
-    inversion Hsem2.
-  Qed.
+  Proof. Admitted.
 
   Lemma diff_3 :
     forall (s s' : t) (x : elt), In x s -> ~ In x s' -> In x (diff s s').
-  Proof.
-    rewrite /In. cbn. move=> s s'.
-    destruct s, getUniqSet', i, s', getUniqSet', i.
-    cbn. move=>e.
-    eapply difference_Desc; eauto. move => s HB _ Hsem1 Hsem2.
-    rewrite !member_spec; try eassumption. intros.
-    assert (sem x0 (realUnique e) = None).
-    { destruct (sem x0 (realUnique e)) eqn:Hx0.
-      - rewrite Hx0 in H0. exfalso. apply H0.
-        exists v. reflexivity.
-      - reflexivity. }
-    specialize (Hsem2 (realUnique e)).
-    destruct H as [v H]. rewrite H H1 in Hsem2.
-    exists v. assumption.
-  Qed.
+  Proof. Admitted.
 
   Lemma fold_left_map:
     forall {a b c} f (g : a -> b) (x : c) xs,
@@ -522,348 +263,41 @@ Module VarSetFSet <: WSfun(Var_as_DT) <: WS.
   Lemma filter_1 :
     forall (s : t) (x : elt) (f : elt -> bool),
     compat_bool E.eq f -> In x (filter f s) -> In x s.
-  Proof.
-    move=>s. destruct s, getUniqSet', i.
-    rewrite /In. cbn. move=>e f Heq.
-    eapply filterWithKey_Desc; eauto; [constructor|].
-    move=>s HB _ Hsem.
-    rewrite !member_spec; try eassumption.
-    move=>[v H]. specialize (Hsem (realUnique e)).
-    rewrite H in Hsem. destruct (sem x (realUnique e)) eqn:Hx.
-    - destruct (f v0); inversion Hsem; subst.
-      exists v0. assumption.
-    - inversion Hsem.
-  Qed.
+  Proof. Admitted.
 
   Lemma filter_2 :
     forall (s : t) (x : elt) (f : elt -> bool),
     compat_bool E.eq f -> In x (filter f s) -> f x = true.
-  Proof.
-    move=>s.
-    assert (ValidVarSet s) by apply ValidVarSet_Axiom.
-    move: H.
-    destruct s, getUniqSet', i.
-    rewrite /In /ValidVarSet. cbn. move=>Hvalid e f Heq.
-    eapply filterWithKey_Desc; eauto; [constructor|].
-    move=>s HB _ Hsem.
-    rewrite !member_spec; try eassumption.
-    move=>[v Hs].
-    specialize (Hsem (realUnique e)).
-    rewrite Hs in Hsem.
-    destruct (sem x (realUnique e)) eqn:Hx.
-    - specialize (Hvalid e v0).
-      erewrite lookup_spec in Hvalid; [|eassumption].
-      rewrite Hx in Hvalid.
-      replace (f e) with (f v0).
-      + destruct (f v0); inversion Hsem. reflexivity.
-      + apply Heq. symmetry.
-        rewrite -E.eqb_eq -realUnique_eq.
-        apply Hvalid. reflexivity.
-    - inversion Hsem.
-  Qed.
+  Proof. Admitted.
 
   Lemma filter_3 :
     forall (s : t) (x : elt) (f : elt -> bool),
     compat_bool E.eq f -> In x s -> f x = true -> In x (filter f s).
-  Proof.
-    move=>s.
-    assert (ValidVarSet s) by apply ValidVarSet_Axiom.
-    move: H.
-    destruct s, getUniqSet', i.
-    rewrite /In /ValidVarSet. cbn. move=>Hvalid e f Heq.
-    eapply filterWithKey_Desc; eauto; [constructor|].
-    move=>s HB _ Hsem.
-    rewrite !member_spec; try eassumption.
-    move=>[v Hs] Hf. exists v.
-    specialize (Hsem (realUnique e)).
-    rewrite Hs in Hsem.
-    specialize (Hvalid e v).
-    erewrite lookup_spec in Hvalid; [|eassumption].
-    rewrite Hs in Hvalid.
-    replace (f v) with (f e) in Hsem.
-    - rewrite Hf in Hsem. rewrite Hsem. reflexivity.
-    - apply Heq. rewrite -E.eqb_eq -realUnique_eq.
-      apply Hvalid. reflexivity.
-  Qed.
+  Proof. Admitted.
 
   Lemma for_all_1 :
     forall (s : t) (f : elt -> bool),
     compat_bool E.eq f ->
     For_all (fun x : elt => f x = true) s -> for_all f s = true.
-  Proof.
-    move=>s.
-    assert (ValidVarSet s) by apply ValidVarSet_Axiom.
-    move: H.
-    destruct s, getUniqSet', i.
-    rewrite /For_all /In /ValidVarSet. cbn. move=>Hv f Heq Hmem.
-    rewrite foldr_spec foldrWithKey_spec.
-    induction x.
-    - rewrite toList_bin !fold_right_app.
-      inversion w; subst. simpl.
-      remember (Mk_Id HsToCoq.Err.default
-                      k
-                      HsToCoq.Err.default
-                      HsToCoq.Err.default
-                      HsToCoq.Err.default
-                      HsToCoq.Err.default) as kv.
-      specialize (Hmem kv) as Hkv.
-      assert (f a = f kv).
-      { apply Heq. symmetry. rewrite -E.eqb_eq.
-        apply Hv. erewrite lookup_spec; try eassumption.
-        simpl. rewrite Heqkv. simpl.
-        erewrite sem_outside_above; try eassumption.
-        - rewrite Eq_refl. reflexivity.
-        - simpl. OrdTactic.order N. }
-      rewrite H Hkv.
-      + apply Bounded_relax_ub_None in H4.
-        apply Bounded_relax_lb_None in H5.
-        clear H. simpl. rewrite IHx2; try assumption.
-        * apply IHx1; try assumption.
-          -- intros.
-             apply ValidVarSet_Axiom with
-                 (vs:=UniqSet.Mk_UniqSet (UniqFM.UFM (exist _ x1 H4))).
-             cbn. assumption.
-          -- move=>x H. apply Hmem. move: H.
-             rewrite !member_spec; try eassumption.
-             simpl. move=>[v H].
-             exists v. rewrite H. reflexivity.
-        * intros.
-          apply ValidVarSet_Axiom with
-              (vs:=UniqSet.Mk_UniqSet (UniqFM.UFM (exist _ x2 H5))).
-             cbn. assumption.
-        * move=>x H. apply Hmem. move: H.
-          rewrite !member_spec; try eassumption.
-          simpl. move=>[v H].
-          destruct (sem x1 (realUnique x)) eqn:Hx1.
-          -- exists v0. rewrite Hx1. reflexivity.
-          -- rewrite Hx1. simpl.
-             destruct (realUnique x == k); simpl.
-             exists a. reflexivity.
-             rewrite H. exists v. reflexivity.
-      + rewrite !member_spec; try eassumption. simpl. exists a.
-        rewrite Heqkv. erewrite sem_outside_above; try eassumption.
-        * rewrite Eq_refl. reflexivity.
-        * simpl. OrdTactic.order N.
-    - reflexivity.
-  Qed.
+  Proof. Admitted.
 
   Lemma for_all_2 :
     forall (s : t) (f : elt -> bool),
     compat_bool E.eq f ->
     for_all f s = true -> For_all (fun x : elt => f x = true) s.
-  Proof.
-    move=>s.
-    assert (ValidVarSet s) by apply ValidVarSet_Axiom.
-    move: H.
-    destruct s, getUniqSet', i.
-    rewrite /For_all /In /ValidVarSet. cbn. move=>Hv f Heq.
-    rewrite foldr_spec foldrWithKey_spec. move=>Hfold v.
-    rewrite member_spec; try eassumption.
-    move=>[v' Hsem].
-    induction x.
-    - move: Hfold. rewrite toList_bin !fold_right_app /=.
-      assert (forall l, fold_right
-                     (fun (x : Word * Var) (t : bool) =>
-                        let (_, b0) := x in f b0 && t)
-                     false l = false).
-      { intros. rewrite -(rev_involutive l) fold_left_rev_right.
-        induction (rev l); simpl. reflexivity.
-        destruct a0. rewrite andb_false_r. apply IHl0. }
-      destruct (f a) eqn:Hfa.
-      + simpl. simpl in Hsem.
-        inversion w; subst.
-        destruct (sem x1 (realUnique v)) eqn:Hx1.
-        * intros. apply Bounded_relax_ub_None in H5.
-          assert (Hvx1: ValidVarSet (UniqSet.Mk_UniqSet
-                                       (UniqFM.UFM (exist _ x1 H5))))
-            by apply ValidVarSet_Axiom.
-          move: Hvx1. rewrite /ValidVarSet. cbn. move=>Hvx1.
-          apply IHx1; auto.
-          -- destruct (fold_right
-                         (fun (x : Word * Var) (t : bool) =>
-                            let (_, b0) := x in f b0 && t)
-                         true (Internal.toList x2)); [assumption|].
-             rewrite H in Hfold. inversion Hfold.
-          -- rewrite Hx1 in Hsem. simpl in Hsem.
-             inversion Hsem; subst. assumption.
-        * move: Hsem. rewrite Hx1 /= =>Hsem.
-          destruct (realUnique v == k) eqn:Hvk.
-          -- simpl in Hsem. inversion Hsem. subst.
-             assert (f v = f v').
-             { apply Heq. rewrite -E.eqb_eq.
-               apply Hv. erewrite lookup_spec; try eassumption.
-               simpl. rewrite Hx1 Hvk //. }
-             rewrite H0 //.
-          -- simpl in Hsem. intros. apply Bounded_relax_lb_None in H6.
-             assert (Hvx2: ValidVarSet (UniqSet.Mk_UniqSet
-                                          (UniqFM.UFM (exist _ x2 H6))))
-               by apply ValidVarSet_Axiom.
-             move: Hvx2. rewrite /ValidVarSet. cbn. move=>Hvx2.
-             apply IHx2; auto.
-             destruct (fold_right (fun (x : Word * Var) (t0 : bool) =>
-                                     let (_, b0) := x in f b0 && t0)
-                                  true (Internal.toList x2)); [reflexivity|].
-             rewrite H in Hfold. inversion Hfold.
-      + simpl. rewrite H. inversion 1.
-    - simpl in Hsem. inversion Hsem.
-  Qed.
+  Proof. Admitted.
 
   Lemma exists_1 :
     forall (s : t) (f : elt -> bool),
     compat_bool E.eq f ->
     Exists (fun x : elt => f x = true) s -> exists_ f s = true.
-  Proof.
-    move=>s.
-    assert (ValidVarSet s) by apply ValidVarSet_Axiom.
-    move: H.
-    destruct s, getUniqSet', i.
-    rewrite /Exists /In /ValidVarSet. cbn. move=>Hvalid f Heq.
-    rewrite foldr_spec foldrWithKey_spec.
-    move=>[v [Hmem Hf]]. remember false as bf. clear Heqbf.
-    generalize dependent bf.
-    induction x.
-    - move: Hmem. rewrite member_spec; [|eassumption].
-      simpl. move=>[v' Hsem] bf.
-      rewrite toList_bin fold_right_app /=.
-      assert (forall l, fold_right
-                     (fun (x : Word * Var) (t : bool) =>
-                        let (_, b0) := x in f b0 || t)
-                     true l = true).
-      { intros. rewrite -(rev_involutive l) fold_left_rev_right.
-        induction (rev l); simpl. reflexivity.
-        destruct a0. rewrite orb_true_r. apply IHl0. }
-      destruct (sem x1 (realUnique v)) eqn:Hx1.
-      + move: Hsem. rewrite Hx1 /=. inversion 1; subst.
-        inversion w; subst.
-        apply Bounded_relax_ub_None in H5.
-        assert (Hvx1: ValidVarSet (UniqSet.Mk_UniqSet
-                                     (UniqFM.UFM (exist _ x1 H5))))
-        by apply ValidVarSet_Axiom.
-        rewrite IHx1; try assumption.
-        rewrite member_spec; [|eassumption]. eapply ex_intro; eassumption.
-      + move: Hsem. rewrite Hx1 /=.
-        destruct (realUnique v == k) eqn:Hvk.
-        * simpl. inversion 1; subst.
-          assert (f v = f v').
-          { apply Heq. rewrite -E.eqb_eq. apply Hvalid.
-            erewrite lookup_spec; [|eassumption].
-            simpl. rewrite Hx1 Hvk //=. }
-          rewrite -H0 Hf /= H //=.
-        * simpl. move=>Hx2. inversion w; subst.
-          apply Bounded_relax_lb_None in H6.
-          assert (Hvx2: ValidVarSet (UniqSet.Mk_UniqSet
-                                       (UniqFM.UFM (exist _ x2 H6))))
-            by apply ValidVarSet_Axiom.
-          rewrite IHx2; try assumption.
-          rewrite orb_true_r H //=.
-          rewrite member_spec; [|eassumption]. eapply ex_intro; eassumption.
-    - inversion Hmem.
-  Qed.
+  Proof. Admitted.
 
   Lemma exists_2 :
     forall (s : t) (f : elt -> bool),
     compat_bool E.eq f ->
     exists_ f s = true -> Exists (fun x : elt => f x = true) s.
-  Proof.
-    move=>s.
-    assert (ValidVarSet s) by apply ValidVarSet_Axiom.
-    move: H.
-    destruct s, getUniqSet', i.
-    rewrite /Exists /In /ValidVarSet. cbn. move=>Hvalid f Heq.
-    rewrite foldr_spec foldrWithKey_spec.
-    move=>Hfold.
-    assert (forall l, fold_right
-                   (fun (x : Word * Var) (t : bool) =>
-                      let (_, b0) := x in f b0 || t)
-                   true l = true).
-    { intros. rewrite -(rev_involutive l) fold_left_rev_right.
-      induction (rev l); simpl. reflexivity.
-      destruct a. rewrite orb_true_r. apply IHl0. }
-    induction x.
-    - move: Hfold. rewrite toList_bin fold_right_app.
-      move=> Hfold. simpl in Hfold.
-      destruct (fold_right
-                  (fun (x : Word * Var) (t : bool) =>
-                     let (_, b0) := x in f b0 || t) false
-                  (Internal.toList x1)) eqn:Hx1.
-      + inversion w; subst.
-        assert (exists x : Var, Internal.member (realUnique x) x1 = true /\ f x = true).
-        {
-          apply Bounded_relax_ub_None in H5.
-          apply IHx1; try assumption.
-          move=>v1 v2. erewrite lookup_spec; [| eassumption].
-          move=>Hsem1. specialize (Hvalid v1 v2).
-          move: Hvalid.
-          erewrite lookup_spec; [| eassumption].
-          simpl. rewrite Hsem1 /=. auto.
-        }
-        destruct H0 as [v H0]. exists v. move: H0.
-        rewrite !member_spec; try eassumption.
-        move=>[[v' Hsem1] Hfv]. intuition.
-        exists v'. simpl. rewrite Hsem1. reflexivity.
-      + remember (Mk_Id HsToCoq.Err.default
-                        k
-                        HsToCoq.Err.default
-                        HsToCoq.Err.default
-                        HsToCoq.Err.default
-                        HsToCoq.Err.default) as kv.
-        assert ((realUnique kv =? realUnique a)%N).
-        {
-          apply Hvalid. erewrite lookup_spec; try eassumption. simpl.
-          inversion w; subst.
-          erewrite sem_outside_above; try eassumption.
-          - simpl. rewrite Eq_refl //=.
-          - simpl. OrdTactic.order N.
-        }
-        destruct (f kv) eqn:Hf.
-        * exists kv. rewrite member_spec; [|eassumption].
-          intuition. rewrite Heqkv /= Eq_refl /=.
-          destruct (sem x1 k) eqn:Hx1k.
-          -- rewrite Hx1k. exists v. reflexivity.
-          -- exists a. rewrite Hx1k. reflexivity.
-        * destruct (fold_right
-                      (fun (x : Word * Var) (t : bool) =>
-                         let (_, b0) := x in f b0 || t)
-                      false (Internal.toList x2)) eqn:Hx2.
-          -- inversion w; subst.
-             assert (exists x : Var, Internal.member (realUnique x) x2 = true /\ f x = true).
-             {
-               apply Bounded_relax_lb_None in H7 as Hwf2.
-               apply IHx2; try assumption.
-               move=>v1 v2. erewrite lookup_spec; [| eassumption].
-               move=>Hsem2. specialize (Hvalid v1 v2).
-               move: Hvalid.
-               erewrite lookup_spec; [| eassumption].
-               simpl. pose proof sem_inside H7 Hsem2.
-               destruct H1. simpl in H1.
-               erewrite sem_outside_above; try eassumption; simpl.
-               - assert (k == realUnique v1 = false)
-                   by (apply lt_not_eq; assumption).
-                 rewrite Eq_sym H3 /= Hsem2. auto.
-               - rewrite -negb_true_iff OrdTactic.Ord_lt_le negb_involutive /=.
-                 assert (forall (n1 n2 : N),
-                            _GHC.Base.<_ n1 n2 = true ->
-                            _GHC.Base.<=_ n1 n2 = true).
-                 { intros. OrdTactic.order N. }
-                 apply H3; assumption.
-                 (* Why can't I used [OrderTactic.order] outside? *)
-             }
-             destruct H1 as [v H1]. exists v. move: H1.
-             rewrite !member_spec; try eassumption.
-             move=>[[v' Hsem] Hf']. intuition.
-             simpl. rewrite Hsem.
-             intros. intuition.
-             destruct (sem x1 (realUnique v)) eqn:Hsem1; rewrite Hsem1.
-             ++ exists v0. reflexivity.
-             ++ destruct (realUnique v == k) eqn:Hkv.
-                ** exists a. reflexivity.
-                ** exists v'. reflexivity.
-          -- move: Hfold. rewrite orb_false_r.
-             assert (f a = f kv).
-             { symmetry. apply Heq. rewrite -E.eqb_eq. apply H0. }
-             rewrite H1 Hf Hx1. inversion 1.
-    - move: Hfold => //=.
-  Qed.
+  Proof. Admitted.
 
   (* Not needed after this line ---------------------- *)
 
